src/cddl/tool/CDDL.Tool.Gen.fst
@@ -115,12 +115,14 @@ let rec compute_wf_typ
     RSuccess (fuel, (f, wf_ast_env_extend_typ_with_weak env name t wt))
   else RFailure (name ^ " is already defined")
 
+
 let produce_validator env wf validator = "
 let _ : unit = _ by (FStar.Tactics.print (\"validator\"); FStar.Tactics.exact (`()))
 [@@normalize_for_extraction (nbe :: T.steps)]
 let "^validator^" = Impl.validate_typ Det.cbor_det_impl "^env^".be_v true _ "^wf
 
 let _pretty : string = "\"_pretty\""
+
 
 let produce_parser0 env env_anc' wf validator parser serializer typename bundle = "
 [@@bundle_attr; bundle_get_impl_type_attr]
@@ -142,15 +144,15 @@ noeq
 %splice[spect_"^typename^"_pretty; spect_"^typename^"_pretty_left; spect_"^typename^"_pretty_right; spect_"^typename^"_pretty_left_right; spect_"^typename^"_pretty_right_left] (FStar.Tactics.PrettifyType.entry "^_pretty^" (`%spect_"^typename^"))
 #pop-options
 inline_for_extraction noextract [@@noextract_to "^krml^"; bundle_attr; bundle_get_impl_type_attr]
-let "^bundle^"'' = bundle_bij "^bundle^"' spect_"^typename^"_pretty_right spect_"^typename^"_pretty_left spect_"^typename^"_pretty_left_right spect_"^typename^"_pretty_right_left (T.eq_sym (specteq"^bundle^" ())) "^typename^"_pretty_right "^typename^"_pretty_left "^typename^"_pretty_left_right "^typename^"_pretty_right_left (T.eq_sym (teq"^bundle^" ()))
+let "^bundle^"'' = bundle_bij "^bundle^"' spect_"^typename^"_pretty_right spect_"^typename^"_pretty_left (T.squash_bij_lemma spect_"^typename^"_pretty_left_right) (T.squash_bij_lemma spect_"^typename^"_pretty_right_left) (T.eq_sym (T.as_squash specteq"^bundle^")) "^typename^"_pretty_right "^typename^"_pretty_left (T.squash_bij_lemma "^typename^"_pretty_left_right) (T.squash_bij_lemma "^typename^"_pretty_right_left) (T.eq_sym (T.as_squash teq"^bundle^"))
 [@@bundle_attr; bundle_get_impl_type_attr]
 let g"^bundle^"'' : Ghost.erased (bundle Det.cbor_det_match) = Ghost.hide "^bundle^"''
 let relteq"^bundle^" () : Lemma (rel "^typename^"_pretty spect_"^typename^"_pretty == rel "^bundle^"''.b_impl_type "^bundle^"''.b_spec_type) by (T.lemma_as_squash(); FStar.Tactics.norm (nbe :: T.bundle_get_rel_steps); FStar.Tactics.trefl ()) = ()
 noextract [@@noextract_to "^krml^"; FStar.Tactics.postprocess_with (fun _ -> FStar.Tactics.norm (nbe :: T.bundle_get_rel_steps); FStar.Tactics.trefl ())]
-let rel_"^typename^" : rel "^typename^"_pretty spect_"^typename^"_pretty = coerce_eq (T.eq_sym (relteq"^bundle^" ())) "^bundle^"''.b_rel
-let releq"^bundle^" () : Lemma (rel_"^typename^" == coerce_eq (T.eq_sym (relteq"^bundle^" ())) "^bundle^"''.b_rel) by (T.lemma_as_squash(); FStar.Tactics.norm (nbe :: T.bundle_get_rel_steps); FStar.Tactics.trefl ()) = ()
+let rel_"^typename^" : rel "^typename^"_pretty spect_"^typename^"_pretty = coerce_eq (T.eq_sym (T.as_squash relteq"^bundle^")) "^bundle^"''.b_rel
+let releq"^bundle^" () : Lemma (rel_"^typename^" == coerce_eq (T.eq_sym (T.as_squash relteq"^bundle^")) "^bundle^"''.b_rel) by (T.lemma_as_squash(); FStar.Tactics.norm (nbe :: T.bundle_get_rel_steps); FStar.Tactics.trefl ()) = ()
 let grelteq"^bundle^" : unit -> Lemma (rel "^typename^"_pretty spect_"^typename^"_pretty == rel g"^bundle^"''.b_impl_type g"^bundle^"''.b_spec_type) = coerce_eq (_ by (FStar.Tactics.norm [delta_only [`%g"^bundle^"''; `%coerce_eq]; primops]; FStar.Tactics.trefl ())) (relteq"^bundle^")
-let greleq"^bundle^" : unit -> Lemma (rel_"^typename^" == coerce_eq (T.eq_sym (grelteq"^bundle^" ())) g"^bundle^"''.b_rel) = coerce_eq (_ by (FStar.Tactics.norm [delta_only [`%g"^bundle^"''; `%coerce_eq]; primops]; FStar.Tactics.trefl ())) (releq"^bundle^")
+let greleq"^bundle^" : unit -> Lemma (rel_"^typename^" == coerce_eq (T.eq_sym (T.as_squash grelteq"^bundle^")) g"^bundle^"''.b_rel) = coerce_eq (_ by (FStar.Tactics.norm [delta_only [`%g"^bundle^"''; `%coerce_eq]; primops]; FStar.Tactics.trefl ())) (releq"^bundle^")
 let specteq"^bundle^"'' () : Lemma ("^bundle^"''.b_spec_type == spect_"^typename^"_pretty) by (T.lemma_as_squash();FStar.Tactics.norm (nbe :: T.bundle_get_spec_type_steps); FStar.Tactics.trefl ()) = ()
 let gspecteq"^bundle^"'' : unit -> Lemma (g"^bundle^"''.b_spec_type == spect_"^typename^"_pretty) = coerce_eq (_ by (FStar.Tactics.norm [delta_only [`%g"^bundle^"''; `%coerce_eq]; primops]; FStar.Tactics.trefl ())) (specteq"^bundle^"'')
 let teq"^bundle^"'' () : Lemma ("^bundle^"''.b_impl_type == "^typename^"_pretty) by (T.lemma_as_squash(); FStar.Tactics.norm (nbe :: T.bundle_get_impl_type_steps); FStar.Tactics.trefl ()) = ()
@@ -494,11 +496,11 @@ let produce_typ_defs
   let anc' : ancillaries_t wenv'.e_sem_env = extend_ancillaries_t anc1.anc wenv'.e_sem_env in
   let msg = "
 let "^source^"_cons () : Lemma (Cons? "^source^") by (T.lemma_as_squash(); T.trefl_or_norm ()) = ()
-let _ : unit = assert (\""^name^"\" == T.pull_name "^source^" ("^source^"_cons ())) by (T.trefl_or_norm ())
+let _ : unit = assert (\""^name^"\" == T.pull_name "^source^" (T.as_squash "^source^"_cons)) by (T.trefl_or_norm ())
 let _ : unit = _ by (FStar.Tactics.print (\"owf'\"); FStar.Tactics.exact (`()))
 let "^source^"_type () : Lemma (CDDL.Spec.AST.Driver.DType? (snd (T.list_hd "^source^" ("^source^"_cons ())))) by (T.lemma_as_squash(); T.trefl_or_norm ()) = ()
 [@@noextract_to "^krml^"; "^opaque_to_smt^"] noextract
-let o"^wf^"' = compute_wf_typ' "^env^".be_ast (T.pull_name "^source^" ("^source^"_cons ())) (_ by (T.trefl_or_norm ())) (T.pull_type "^source^" ("^source^"_cons ()) ("^source^"_type ())) "^fuel^"
+let o"^wf^"' = compute_wf_typ' "^env^".be_ast (T.pull_name "^source^" ("^source^"_cons ())) (_ by (T.trefl_or_norm ())) (T.pull_type "^source^" (T.as_squash "^source^"_cons) (T.as_squash "^source^"_type)) "^fuel^"
 let _ : unit = _ by (FStar.Tactics.print (\"owf\"); FStar.Tactics.exact (`()))
 [@@FStar.Tactics.postprocess_with (fun _ -> FStar.Tactics.norm [delta; zeta; iota; primops]; FStar.Tactics.trefl ()); noextract_to "^krml^"; "^opaque_to_smt^"; "^opaque_to_smt^"] noextract
 let o"^wf^" = o"^wf^"'
@@ -605,12 +607,12 @@ module SZ = FStar.SizeT
 let option_source = CDDL.Tool.Plugin.parse ["^filenames^"]
 let option_source_some () : Lemma (Some? option_source) by (T.lemma_as_squash(); FStar.Tactics.norm [delta; iota; primops]; FStar.Tactics.trefl ()) = ()
 [@@FStar.Tactics.postprocess_with (fun _ -> FStar.Tactics.norm [delta; iota; primops]; FStar.Tactics.trefl ()); noextract_to "^krml^"; "^opaque_to_smt^"] noextract
-let source = T.get_option_some option_source (option_source_some ())
+let source = T.get_option_some option_source (T.as_squash option_source_some)
 [@@FStar.Tactics.postprocess_with (fun _ -> FStar.Tactics.norm [delta; zeta; iota; primops]; FStar.Tactics.trefl ()); noextract_to "^krml^"; "^opaque_to_smt^"] noextract
 let option_sorted_source = topological_sort source
 let option_sorted_source_some () : Lemma (Some? option_sorted_source) by (T.lemma_as_squash(); FStar.Tactics.norm [delta; iota; primops]; FStar.Tactics.trefl ()) = ()
 [@@FStar.Tactics.postprocess_with (fun _ -> FStar.Tactics.norm [delta; zeta; iota; primops]; FStar.Tactics.trefl ()); noextract_to "^krml^"; base_attr; "^opaque_to_smt^"] noextract
-let sorted_source0 = T.get_option_some option_sorted_source (option_sorted_source_some ())
+let sorted_source0 = T.get_option_some option_sorted_source (T.as_squash option_sorted_source_some)
 [@@noextract_to "^krml^"; sem_attr; bundle_attr; "^opaque_to_smt^"] noextract
 let env0 : bundle_env Det.cbor_det_match = empty_bundle_env _
 [@@noextract_to "^krml^"; sem_attr; bundle_attr; "^opaque_to_smt^"] noextract
